final project/ConstantFolding.v
@@ -1,0 +1,597 @@
+(**
+*  CS386L Programming Languages
+* Final project
+* Tian Zhang (tz3272)
+* Brief Introduction:
+*     For the final project, I am working on partial evaluation, and 
+      all the work is based on Maps, Imp in class. I got some idea from
+      the book, as 
+*)
+
+
+Require Import Coq.Bool.Bool.
+Require Import Coq.Arith.Arith.
+Require Import Coq.Arith.EqNat.
+Require Import Coq.omega.Omega.
+Require Import Coq.Lists.List.
+Require Import Coq.Logic.FunctionalExtensionality.
+Import ListNotations.
+Require Import Maps.
+Require Import Imp.
+
+
+(* ################################################################# *)
+(** * Constant Folding*)
+
+(** before partial evalation, the first part I want to implement
+  a more simple idea, constant folding
+
+  An expression is constant when it contains no variable
+  references. Constant folding is an optimization that finds constant
+  expressions and replaces them by their values. 
+*)
+
+Fixpoint fold_constants_aexp (a : aexp) : aexp :=
+  match a with
+  | ANum n       => ANum n
+  | AId i        => AId i
+  | APlus a1 a2  =>
+    match (fold_constants_aexp a1, fold_constants_aexp a2)
+    with
+    | (ANum n1, ANum n2) => ANum (n1 + n2)
+    | (a1', a2') => APlus a1' a2'
+    end
+  | AMinus a1 a2 =>
+    match (fold_constants_aexp a1, fold_constants_aexp a2)
+    with
+    | (ANum n1, ANum n2) => ANum (n1 - n2)
+    | (a1', a2') => AMinus a1' a2'
+    end
+  | AMult a1 a2  =>
+    match (fold_constants_aexp a1, fold_constants_aexp a2)
+    with
+    | (ANum n1, ANum n2) => ANum (n1 * n2)
+    | (a1', a2') => AMult a1' a2'
+    end
+  end.
+
+(** Example, fold 1 + 2 => 3 *)
+Example fold_aexp_ex1 :
+    fold_constants_aexp
+      (AMult (APlus (ANum 1) (ANum 2)) (AId X))
+  = AMult (ANum 3) (AId X).
+Proof. reflexivity. Qed.
+
+(** we can also fold boolean expression , if we find constant boolean expression
+    we can evaluate in place *)
+
+Fixpoint fold_constants_bexp (b : bexp) : bexp :=
+  match b with
+  | BTrue        => BTrue
+  | BFalse       => BFalse
+  | BEq a1 a2  =>
+    match (fold_constants_aexp a1, fold_constants_aexp a2)
+    with
+    | (ANum n1, ANum n2) =>
+        if beq_nat n1 n2 then BTrue else BFalse
+    | (a1', a2') =>
+        BEq a1' a2'
+    end
+  | BLe a1 a2  =>
+    match (fold_constants_aexp a1, fold_constants_aexp a2)
+    with
+    | (ANum n1, ANum n2) =>
+        if leb n1 n2 then BTrue else BFalse
+    | (a1', a2') =>
+        BLe a1' a2'
+    end
+  | BNot b1  =>
+    match (fold_constants_bexp b1) with
+    | BTrue => BFalse
+    | BFalse => BTrue
+    | b1' => BNot b1'
+    end
+  | BAnd b1 b2  =>
+    match (fold_constants_bexp b1, fold_constants_bexp b2)
+    with
+    | (BTrue, BTrue) => BTrue
+    | (BTrue, BFalse) => BFalse
+    | (BFalse, BTrue) => BFalse
+    | (BFalse, BFalse) => BFalse
+    | (b1', b2') => BAnd b1' b2'
+    end
+  end.
+
+Example fold_bexp_ex1 :
+    fold_constants_bexp (BAnd BTrue (BNot (BAnd BFalse BTrue)))
+  = BTrue.
+Proof. reflexivity. Qed.
+
+(** the next step is to fold constant in command*)
+Fixpoint fold_constants_com (c : com) : com :=
+  match c with
+  | SKIP      =>
+      SKIP
+  | i ::= a  =>
+      CAss i (fold_constants_aexp a)
+  | c1 ;; c2  =>
+      (fold_constants_com c1) ;; (fold_constants_com c2)
+  | IFB b THEN c1 ELSE c2 FI =>
+      match fold_constants_bexp b with
+      | BTrue => fold_constants_com c1
+      | BFalse => fold_constants_com c2
+      | b' => IFB b' THEN fold_constants_com c1
+                     ELSE fold_constants_com c2 FI
+      end
+  | WHILE b DO c END =>
+      match fold_constants_bexp b with
+      | BTrue => WHILE BTrue DO SKIP END
+      | BFalse => SKIP
+      | b' => WHILE b' DO (fold_constants_com c) END
+      end
+  end.
+  
+(** Example *)
+Example fold_com_ex1 :
+  fold_constants_com
+    (* Original program: *)
+    (X ::= APlus (ANum 4) (ANum 5);;
+     Y ::= AMinus (AId X) (ANum 3);;
+     IFB BEq (AMinus (AId X) (AId Y))
+             (APlus (ANum 2) (ANum 4)) THEN
+       SKIP
+     ELSE
+       Y ::= ANum 0
+     FI;;
+     IFB BLe (ANum 0)
+             (AMinus (ANum 4) (APlus (ANum 2) (ANum 1))) 
+     THEN
+       Y ::= ANum 0
+     ELSE
+       SKIP
+     FI;;
+     WHILE BEq (AId Y) (ANum 0) DO
+       X ::= APlus (AId X) (ANum 1)
+     END)
+  = (* After constant folding: *)
+    (X ::= ANum 9;;
+     Y ::= AMinus (AId X) (ANum 3);;
+     IFB BEq (AMinus (AId X) (AId Y)) (ANum 6) THEN
+       SKIP
+     ELSE
+       (Y ::= ANum 0)
+     FI;;
+     Y ::= ANum 0;;
+     WHILE BEq (AId Y) (ANum 0) DO
+       X ::= APlus (AId X) (ANum 1)
+     END).
+Proof. reflexivity. Qed.
+
+(** Now we have constant folding, we need to prove that, after folding,
+  the program is correct*)
+  
+(** Here is some definition in equiv.v to help prove that constant 
+  folding is correct*)
+  
+  
+(** First, we need to introduce the behaviorally equivalent 
+    that two aexp or bexp are behaviorally equivalent if they
+    evaluate to the same result in every state. *)
+
+Definition aequiv (a1 a2 : aexp) : Prop :=
+  forall (st:state),
+    aeval st a1 = aeval st a2.
+
+Definition bequiv (b1 b2 : bexp) : Prop :=
+  forall (st:state),
+    beval st b1 = beval st b2.
+
+
+Definition cequiv (c1 c2 : com) : Prop :=
+  forall (st st' : state),
+    (c1 / st \\ st') <-> (c2 / st \\ st').
+
+(** ** Behavioral Equivalence Is an Equivalence
+    the equivalence can be proved by reflexive,
+    symmetric, and transitive. *)
+
+Lemma refl_aequiv : forall (a : aexp), aequiv a a.
+Proof.
+  intros a st. reflexivity.  Qed.
+
+Lemma sym_aequiv : forall (a1 a2 : aexp),
+  aequiv a1 a2 -> aequiv a2 a1.
+Proof.
+  intros a1 a2 H. intros st. symmetry. apply H.  Qed.
+
+Lemma trans_aequiv : forall (a1 a2 a3 : aexp),
+  aequiv a1 a2 -> aequiv a2 a3 -> aequiv a1 a3.
+Proof.
+  unfold aequiv. intros a1 a2 a3 H12 H23 st.
+  rewrite (H12 st). rewrite (H23 st). reflexivity.  Qed.
+
+Lemma refl_bequiv : forall (b : bexp), bequiv b b.
+Proof.
+  unfold bequiv. intros b st. reflexivity.  Qed.
+
+Lemma sym_bequiv : forall (b1 b2 : bexp),
+  bequiv b1 b2 -> bequiv b2 b1.
+Proof.
+  unfold bequiv. intros b1 b2 H. intros st. symmetry. apply H.  Qed.
+
+Lemma trans_bequiv : forall (b1 b2 b3 : bexp),
+  bequiv b1 b2 -> bequiv b2 b3 -> bequiv b1 b3.
+Proof.
+  unfold bequiv. intros b1 b2 b3 H12 H23 st.
+  rewrite (H12 st). rewrite (H23 st). reflexivity.  Qed.
+
+Lemma refl_cequiv : forall (c : com), cequiv c c.
+Proof.
+  unfold cequiv. intros c st st'. apply iff_refl.  Qed.
+
+Lemma sym_cequiv : forall (c1 c2 : com),
+  cequiv c1 c2 -> cequiv c2 c1.
+Proof.
+  unfold cequiv. intros c1 c2 H st st'.
+  assert (c1 / st \\ st' <-> c2 / st \\ st') as H'.
+  { (* Proof of assertion *) apply H. }
+  apply iff_sym. assumption.
+Qed.
+
+Lemma iff_trans : forall (P1 P2 P3 : Prop),
+  (P1 <-> P2) -> (P2 <-> P3) -> (P1 <-> P3).
+Proof.
+  intros P1 P2 P3 H12 H23.
+  inversion H12. inversion H23.
+  split; intros A.
+    apply H1. apply H. apply A.
+    apply H0. apply H2. apply A.  Qed.
+
+Lemma trans_cequiv : forall (c1 c2 c3 : com),
+  cequiv c1 c2 -> cequiv c2 c3 -> cequiv c1 c3.
+Proof.
+  unfold cequiv. intros c1 c2 c3 H12 H23 st st'.
+  apply iff_trans with (c2 / st \\ st'). apply H12. apply H23.  Qed.
+
+(** Prove that adding a SKIP after a command results in an
+    equivalent program *)
+    
+Theorem IFB_true: forall b c1 c2,
+     bequiv b BTrue  ->
+     cequiv
+       (IFB b THEN c1 ELSE c2 FI)
+       c1.
+Proof.
+  intros b c1 c2 Hb.
+  split; intros H.
+  - (* -> *)
+    inversion H; subst.
+    + (* b evaluates to true *)
+      assumption.
+    + (* b evaluates to false (contradiction) *)
+      unfold bequiv in Hb. simpl in Hb.
+      rewrite Hb in H5.
+      inversion H5.
+  - (* <- *)
+    apply E_IfTrue; try assumption.
+    unfold bequiv in Hb. simpl in Hb.
+    rewrite Hb. reflexivity.  Qed.
+
+Theorem IFB_false: forall b c1 c2,
+  bequiv b BFalse  ->
+  cequiv 
+    (IFB b THEN c1 ELSE c2 FI) 
+    c2.
+Proof.
+  intros b c1 c2 Hb.
+  split; intros H.
+  - (* -> *)
+    inversion H; subst.
+    + (* b => true *)
+    unfold bequiv in Hb.
+    rewrite Hb in H5. inversion H5.
+    + (* b => false *)
+    assumption.
+  - (* <- *)
+    apply E_IfFalse.
+    unfold bequiv in Hb.
+    simpl in Hb. apply Hb.
+    assumption.
+Qed.
+
+(** A loop whose guard is equivalent to BFalse is equivalent to SKIP,
+    while a loop whose guard is equivalent to [BTrue] is equivalent to
+    WHILE BTrue DO SKIP END  *)
+
+Theorem WHILE_false : forall b c,
+     bequiv b BFalse ->
+     cequiv
+       (WHILE b DO c END)
+       SKIP.
+Proof.
+  intros b c Hb. split; intros H.
+  - (* -> *)
+    inversion H; subst.
+    + (* E_WhileEnd *)
+      apply E_Skip.
+    + (* E_WhileLoop *)
+      rewrite Hb in H2. inversion H2.
+  - (* <- *)
+    inversion H; subst.
+    apply E_WhileEnd.
+    rewrite Hb.
+    reflexivity.  Qed.
+    
+Lemma WHILE_true_nonterm : forall b c st st',
+     bequiv b BTrue ->
+     ~( (WHILE b DO c END) / st \\ st' ).
+Proof.
+  (* WORKED IN CLASS *)
+  intros b c st st' Hb.
+  intros H.
+  remember (WHILE b DO c END) as cw eqn:Heqcw.
+  induction H;
+    (* Most rules don't apply, and we can rule them out
+       by inversion *)
+    inversion Heqcw; subst; clear Heqcw.
+  (* The two interesting cases are the ones for WHILE loops: *)
+  - (* E_WhileEnd *) (* contradictory -- b is always true! *)
+    unfold bequiv in Hb.
+    (* [rewrite] is able to instantiate the quantifier in [st] *)
+    rewrite Hb in H. inversion H.
+  - (* E_WhileLoop *) (* immediate from the IH *)
+    apply IHceval2. reflexivity.  Qed.
+
+Theorem ex_falso_quodlibet : forall (P:Prop), False -> P.
+Proof.
+  intros. inversion H.
+Qed.
+
+Lemma skip_state : forall st st',
+                     SKIP / st \\ st' -> st = st'.
+Proof.
+  intros.
+  inversion H. subst.
+  reflexivity.
+Qed.
+
+Theorem WHILE_true: forall b c,
+     bequiv b BTrue  ->
+     cequiv 
+       (WHILE b DO c END)
+       (WHILE BTrue DO SKIP END).
+Proof.
+  intros.
+  intros st st'. split.
+  - (* -> *) 
+    intros.
+    apply WHILE_true_nonterm with (c:=c) (st:=st) (st':=st') in H.
+    apply ex_falso_quodlibet.
+    apply H in H0. assumption.
+  - (* <- *)
+  intros.
+  remember (WHILE BTrue DO SKIP END).
+  induction H0; inversion Heqc0. 
+    + (* E_WhileEnd *)
+  subst. simpl in H0. inversion H0.
+    + (* E_WhileLoop *)
+  subst.
+  clear IHceval1.
+  rename H0_ into Hst.
+  apply skip_state in Hst.
+  rewrite Hst.
+  apply IHceval2.
+  assumption.
+Qed.
+
+(** ** Behavioral Equivalence Is a Congruence *)
+
+(** behavioral equivalence is also a congruence
+    The equivalence of two subprograms implies the
+    equivalence of the larger programs in which they are embedded *)
+
+Theorem CAss_congruence : forall i a1 a1',
+  aequiv a1 a1' ->
+  cequiv (CAss i a1) (CAss i a1').
+Proof.
+  intros i a1 a2 Heqv st st'.
+  split; intros Hceval.
+  - (* -> *)
+    inversion Hceval. subst. apply E_Ass.
+    rewrite Heqv. reflexivity.
+  - (* <- *)
+    inversion Hceval. subst. apply E_Ass.
+    rewrite Heqv. reflexivity.  
+Qed.
+
+Theorem CWhile_congruence : forall b1 b1' c1 c1',
+  bequiv b1 b1' -> cequiv c1 c1' ->
+  cequiv (WHILE b1 DO c1 END) (WHILE b1' DO c1' END).
+Proof.
+  (* WORKED IN CLASS *)
+  unfold bequiv,cequiv.
+  intros b1 b1' c1 c1' Hb1e Hc1e st st'.
+  split; intros Hce.
+  - (* -> *)
+    remember (WHILE b1 DO c1 END) as cwhile
+      eqn:Heqcwhile.
+    induction Hce; inversion Heqcwhile; subst.
+    + (* E_WhileEnd *)
+      apply E_WhileEnd. rewrite <- Hb1e. apply H.
+    + (* E_WhileLoop *)
+      apply E_WhileLoop with (st' := st').
+      * (* show loop runs *) rewrite <- Hb1e. apply H.
+      * (* body execution *)
+        apply (Hc1e st st').  apply Hce1.
+      * (* subsequent loop execution *)
+        apply IHHce2. reflexivity.
+  - (* <- *)
+    remember (WHILE b1' DO c1' END) as c'while
+      eqn:Heqc'while.
+    induction Hce; inversion Heqc'while; subst.
+    + (* E_WhileEnd *)
+      apply E_WhileEnd. rewrite -> Hb1e. apply H.
+    + (* E_WhileLoop *)
+      apply E_WhileLoop with (st' := st').
+      * (* show loop runs *) rewrite -> Hb1e. apply H.
+      * (* body execution *)
+        apply (Hc1e st st').  apply Hce1.
+      * (* subsequent loop execution *)
+        apply IHHce2. reflexivity.  Qed.
+
+
+Theorem CSeq_congruence : forall c1 c1' c2 c2',
+  cequiv c1 c1' -> cequiv c2 c2' ->
+  cequiv (c1;;c2) (c1';;c2').
+Proof.
+  intros. unfold cequiv. split; intros He.
+  - (* <- *)
+  unfold cequiv in *. inversion He. subst.
+  apply H with (st':=st'0) in H3.
+  apply H0 with (st:=st'0) in H6.
+  apply E_Seq with (st':=st'0). assumption.
+  assumption.
+  - (* -> *)
+  unfold cequiv in *.
+  inversion He. subst.
+  apply H with (st':=st'0) in H3.
+  apply H0 with (st:=st'0) in H6.
+  apply E_Seq with (st':=st'0).
+  assumption.
+  assumption.
+Qed.
+
+Theorem CIf_congruence : forall b b' c1 c1' c2 c2',
+  bequiv b b' -> cequiv c1 c1' -> cequiv c2 c2' ->
+  cequiv (IFB b THEN c1 ELSE c2 FI)
+         (IFB b' THEN c1' ELSE c2' FI).
+Proof.
+  intros.
+  unfold cequiv.
+  split; intro He.
+  - (* -> *)
+  unfold cequiv in *.
+  unfold bequiv in H.
+  inversion He; subst.
+    + (* b => true *)
+    apply E_IfTrue. rewrite H in H7. assumption.
+    rewrite H0 in H8. assumption.
+    + (* b => false *)
+    apply E_IfFalse. rewrite H in H7. assumption.
+    rewrite H1 in H8. assumption.
+  - (* <- *)
+  unfold cequiv in *.
+  unfold bequiv in H.
+  symmetry in H.
+  inversion He; subst.
+     + (* b => true *)
+  apply E_IfTrue. rewrite H in H7. assumption.
+  rewrite <- H0 in H8. assumption.
+     + (* b => false *)
+  apply E_IfFalse. rewrite H in H7. assumption.
+  rewrite <- H1 in H8. assumption.
+Qed.
+
+
+(** A program transformation is _sound_ if it preserves the
+    behavior of the original program. *)
+
+Definition atrans_sound (atrans : aexp -> aexp) : Prop :=
+  forall (a : aexp),
+    aequiv a (atrans a).
+
+Definition btrans_sound (btrans : bexp -> bexp) : Prop :=
+  forall (b : bexp),
+    bequiv b (btrans b).
+
+Definition ctrans_sound (ctrans : com -> com) : Prop :=
+  forall (c : com),
+    cequiv c (ctrans c).
+
+(** The prove has 3 parts, for aexp, bexp and command *)
+    
+Theorem fold_constants_aexp_sound :
+  atrans_sound fold_constants_aexp.
+Proof.
+  unfold atrans_sound. intros a. unfold aequiv. intros st.
+  induction a; simpl;
+    try reflexivity;
+    try (destruct (fold_constants_aexp a1);
+         destruct (fold_constants_aexp a2);
+         rewrite IHa1; rewrite IHa2; reflexivity). 
+Qed.
+
+
+
+Theorem fold_constants_bexp_sound:
+  btrans_sound fold_constants_bexp.
+Proof.
+  unfold btrans_sound. intros b. unfold bequiv. intros st.
+  induction b;
+   
+    try reflexivity.
+  - rename a into a1. rename a0 into a2. simpl.
+    remember (fold_constants_aexp a1) as a1' eqn:Heqa1'.
+    remember (fold_constants_aexp a2) as a2' eqn:Heqa2'.
+    replace (aeval st a1) with (aeval st a1') by
+       (subst a1'; rewrite <- fold_constants_aexp_sound; reflexivity).
+    replace (aeval st a2) with (aeval st a2') by
+       (subst a2'; rewrite <- fold_constants_aexp_sound; reflexivity).
+    destruct a1'; destruct a2'; try reflexivity.
+    simpl. destruct (beq_nat n n0); reflexivity.
+  - (* BLe *)
+    rename a into a1. rename a0 into a2. simpl.
+    remember (fold_constants_aexp a1) as a1' eqn:Heqa1'.
+    remember (fold_constants_aexp a2) as a2' eqn:Heqa2'.
+    replace (aeval st a1) with (aeval st a1') by
+      (subst a1'; rewrite <- fold_constants_aexp_sound; reflexivity).
+    replace (aeval st a2) with (aeval st a2') by
+      (subst a2'; rewrite <- fold_constants_aexp_sound; reflexivity).
+    destruct a1'; destruct a2'; auto.
+    simpl. destruct ( n <=? n0); auto.
+  - (* BNot *)
+    simpl. remember (fold_constants_bexp b) as b' eqn:Heqb'.
+    rewrite IHb.
+    destruct b'; reflexivity.
+  - (* BAnd *)
+    simpl.
+    remember (fold_constants_bexp b1) as b1' eqn:Heqb1'.
+    remember (fold_constants_bexp b2) as b2' eqn:Heqb2'.
+    rewrite IHb1. rewrite IHb2.
+    destruct b1'; destruct b2'; simpl; try reflexivity
+    ; eauto using andb_true_l, andb_true_r, andb_false_l, andb_false_r.
+Qed.
+
+
+
+Theorem fold_constants_com_sound :
+  ctrans_sound fold_constants_com.
+Proof.
+  unfold ctrans_sound. intros c.
+  induction c; simpl.
+  - (* SKIP *) apply refl_cequiv.
+  - (* ::= *) apply CAss_congruence.
+              apply fold_constants_aexp_sound.
+  - (* ;; *) apply CSeq_congruence; assumption.
+  - (* IFB *)
+    assert (bequiv b (fold_constants_bexp b)). {
+      apply fold_constants_bexp_sound. }
+    destruct (fold_constants_bexp b) eqn:Heqb;
+      try (apply CIf_congruence; assumption).
+
+    + (* b always true *)
+      apply trans_cequiv with c1; try assumption.
+      apply IFB_true; assumption.
+    + (* b always false *)
+      apply trans_cequiv with c2; try assumption.
+      apply IFB_false; assumption.
+  - (* WHILE *)
+    assert (bequiv b (fold_constants_bexp b)).
+    apply fold_constants_bexp_sound.
+    destruct (fold_constants_bexp b) eqn:Hb; try (apply CWhile_congruence; assumption; assumption).
+    apply WHILE_true with (c:=c) in H.
+    assumption.
+    apply WHILE_false with (c:=c) in H.
+    assumption.
+Qed.
+
