final project/README.md
@@ -1,0 +1,7 @@
+# CS386L_PL_coq
+Course project for CS386L programming language, using coq language
+Tian Zhang ( tz3272 )
+
+* ConstantFolding.v : implement constant folding for Imp language
+* PartialEvaluation.v : implement partial evaluation on constant folding.
+
